Fixed the set syntax

Charge!/src/Charge/Tactics/Rtac/Red.v
@@ -24,29 +24,29 @@ Section Red.
   Context {FVAp : PartialView func (ap_func typ)}.
   Context {Expr_expr : Expr typ (expr typ func)}.
 
-  Definition pointwise_redF (f : typ -> expr typ func -> expr typ func) : 
+  Definition pointwise_redF (f : typ -> expr typ func -> expr typ func) (g : typ -> typ) : 
     ptrn (expr typ func) (expr typ func)  :=
     Eval compute in 
-      por (bil_pointwise_red f (fun x => x)) 
-          (por (embed_pointwise_red f (fun x => x)) 
+      por (bil_pointwise_red f g) 
+          (por (embed_pointwise_red f g) 
                (por (red_ap_ptrn f)
-                    (il_pointwise_red f (fun x => x)))).
+                    (il_pointwise_red f g))).
 
-  Fixpoint pointwise_red_aux (s : expr typ func) (t : typ) (e : expr typ func) {struct e} : expr typ func :=
-    run_ptrn (pointwise_redF (pointwise_red_aux s)) (App e s) e.
+  Fixpoint pointwise_red_aux (s : expr typ func) (g : typ -> typ) (t : typ) (e : expr typ func) {struct e} : expr typ func :=
+    run_ptrn (pointwise_redF (pointwise_red_aux s g) g) (App e s) e.
 
-  Definition pointwise_red (s e : expr typ func) := pointwise_red_aux s tyProp e.
+  Definition pointwise_red (t : typ) (s e : expr typ func) (g : typ -> typ) := pointwise_red_aux s g t e.
 
-  Definition red_entails_lhs :=
+  Definition red_entails_lhs (g : typ -> typ) :=
     pmap (fun t' => let '(t, (p, s), r) := t' in 
-    		 mkEntails t (pointwise_red s p) r)
+    		 mkEntails t (pointwise_red t s p g) r)
          (ptrnEntails get (Ptrns.app get get) get).
 
-  Definition RED_ENTAILS : rtac typ (expr typ func) :=
+  Definition RED_ENTAILS (g : typ -> typ) : rtac typ (expr typ func) :=
     fun c s e =>
-      run_ptrn (pmap (fun e => More s (GGoal e)) red_entails_lhs) Fail e.
+      run_ptrn (pmap (fun e' => More s (GGoal e')) (red_entails_lhs g)) Fail e.
       
-  Lemma RED_ENTAILS_sound : rtac_sound RED_ENTAILS.
+  Lemma RED_ENTAILS_sound (g : typ -> typ) : rtac_sound (RED_ENTAILS g).
   Proof.
     admit.
   Admitted.
